\documentclass[12pt]{article}

\usepackage{amsmath}
\usepackage{amsfonts}

\newcommand{\comment}[1]{}

\newcommand{\lr}[1]{ \left( #1 \right) }
\newcommand{\lrs}[1]{ \left[ #1 \right] }
\newcommand{\lrc}[1]{ \left\{ #1 \right\} }
\newcommand{\vev}[1]{ \langle \, #1 \, \rangle }

\newcommand{\Tr}{ {\rm Tr} \, }
\newcommand{\tr}{ {\rm Tr} \, }
\newcommand{\re}{ {\rm Re} \, }
\newcommand{\im}{ {\rm Im} \, }
\renewcommand{\Re}{ {\rm Re} \, }
\renewcommand{\Im}{ {\rm Im} \, }

\newcommand{\rvac}{ \, | 0 \rangle }
\newcommand{\lvac}{ \langle 0 | \, }
\newcommand{\ket}[1]{ \, | #1 \rangle }
\newcommand{\bra}[1]{ \langle #1 | \, }

\newcommand{\diag}[1]{ {\rm diag} \, \left( #1 \right) }
\newcommand{\const}{ {\rm const}}
\renewcommand{\det}[1]{ {\rm det} \left( #1 \right) }

\newcommand{\sign}{ {\rm sign} \,  }
\newcommand{\sh}{ {\rm sh} \,  }
\newcommand{\ch}{ {\rm ch} \,  }
\renewcommand{\th}{ {\rm th} \,  }
\newcommand{\hodge}{{}^{*}}
\newcommand{\expa}[1]{ \exp{\left( #1 \right)} }
\newcommand{\abs}[1]{| #1 |}

\begin{document}

\section{Perturbative expansion of the Jacobian for the exponential mapping $g = e^{i \alpha \phi}$}
\label{sec:exp_J_pert}

 The starting point for this derivation is the explicit expression for the Jacobian of this mapping, given in terms of eigenvalues $\phi_i$ of the matrix $\phi$ (see \cite{Buividovich:15:3}):
\begin{eqnarray}
\label{SUN_haar_measure_phi}
 \int\limits_{U\lr{N}} dg
 =
 \const \, \int d\phi
 \prod\limits_{i > j}
 \frac{\sin^2\lr{\frac{\alpha \lr{\phi_i - \phi_j}}{2}}}{\lr{\phi_i - \phi_j}^2}
 = \nonumber \\ =
 \const \, \int d\phi
 \expa{\frac{1}{2} \sum\limits_{i \neq j} \ln\lr{\frac{\sin^2\lr{\frac{\alpha \lr{\phi_i - \phi_j}}{2}} }{\lr{\phi_i - \phi_j}^2}} } .
\end{eqnarray}
First we define $x_{ij} = \alpha\lr{\phi_i - \phi_j}$ and use the following expansion:
\begin{eqnarray}
\label{sinxx_expansion}
 -\frac{1}{2} \ln \frac{4 \sin^2\lr{x/2}}{x^2} =
 \sum\limits_{k=1}^{+\infty} \mathcal{J}_k x^{2 k}
 = \nonumber \\ =
 \frac{x^2}{24}+\frac{x^4}{2880}+\frac{x^6}{181440}+\frac{x^8}{9676800}+\frac{x^{10}}{479001600} + \ldots
\end{eqnarray}
In order to derive the Schwinger-Dyson equations, now we have to express the argument of the exponential in the second line of (\ref{SUN_haar_measure_phi}) in terms of single-trace operators.
To this end we write
\begin{eqnarray}
\label{phiiphij2traces}
 \sum\limits_{i \neq j} \lr{\phi_i - \phi_j}^k =
 \sum\limits_{l=0}^k \frac{k!}{l! \lr{k - l}!}
 \sum\limits_{i,j} \lr{-\phi_j}^l \phi_i^k
 = \nonumber \\ =
 \sum\limits_{l=0}^k \frac{k!}{l! \lr{k - l}!} \lr{-1}^l \tr\lr{\phi^l} \tr\lr{\phi^k}
\end{eqnarray}
Combining this formula with (\ref{sinxx_expansion}), we get finally $\int\limits_{U\lr{N}} dg
 = \const \, \int d\phi \expa{ - S\lrs{\phi}}$, where
\begin{eqnarray}
\label{SUN_Jacobian_action}
 S\lrs{\phi} = \sum\limits_{k=1}^{+\infty}
 \mathcal{J}_k \alpha^{2 k}
 \sum\limits_{l=0}^k \frac{\lr{2 k}!}{\lr{2 l}! \lr{2 k - 2 l}!} \tr\lr{\phi^{2 l}} \tr\lr{\phi^{2k - 2l}}
  = \nonumber \\ =
 N \frac{\alpha^2}{12} \tr\phi^2
 + \sum\limits_{k=2}^{+\infty}
 \mathcal{J}_k
 \sum\limits_{l=0}^k \frac{\lr{2 k}!}{\lr{2 l}! \lr{2 k - 2 l}!} \tr\lr{\phi^{2 l}} \tr\lr{\phi^{2k - 2l}}
 = \nonumber \\ =
 N \frac{\alpha^2}{12} \tr\phi^2
 +
 \sum\limits_{k=2}^{+\infty} \alpha^{2 k} 2 \mathcal{J}_k \tr{\phi^{2 k}}
 +
 \sum\limits_{k=2}^{+\infty} \alpha^{2 k} \sum\limits_{l=1}^{k-1}
 \mathcal{J}_{k,l} \tr\lr{\phi^{2 l}} \tr\lr{\phi^{2k - 2l}} .
\end{eqnarray}

\section{PCM with exponential mapping}

It is convenient to rewrite the interacting part of the action as
\begin{eqnarray}
\label{pcm_action_int}
 S_I\lrs{\phi_x}
 = \sum\limits_{k=1}^{+\infty} \lr{- \alpha^2}^{k} S_I^{\lr{2k+2}}\lrs{\phi_x} ,
 \nonumber \\
 S_I^{\lr{2k+2}}\lrs{\phi_x} =
 \left(
  \frac{1}{2} \sum\limits_{l=1}^{2 k + 1} \frac{\lr{-1}^{l-1}}{\lr{2 k + 2 - l}! \, l!}
  \sum\limits_{x,y} D_{x y} \tr\lr{\phi_x^{2 k + 2 - l} \phi_y^l }
   + \right. \nonumber \\ \left. +
  \lr{-1}^{k} \lambda \, \mathcal{J}_{k+1} \tr\lr{\phi_x^{2 k+2}}
  +
 \lr{-1}^{k} \frac{\lambda}{2} \, \sum\limits_{l=1}^{k} \mathcal{J}_{k+1,l} \tr\lr{\phi_x^{2 l}} \tr\lr{\phi_x^{2 k + 2 - 2 l}}
  \right)
\end{eqnarray}
The quartic part of the action reads in explicit form:
\begin{eqnarray}
\label{pcm_action_int_quartic}
 S_I^{\lr{4}}\lrs{\phi_x}
 = 
 \frac{1}{6} \sum\limits_{x, y} D_{x y} \tr\lr{\phi_x^3 \phi_y}
 -
 \frac{1}{8} \sum\limits_{x, y} D_{x y} \tr\lr{\phi_x^2 \phi_y^2}
 - \nonumber \\ -
 \frac{\lambda}{2880} \sum\limits_x \tr\lr{\phi_x^4}
 -
 \frac{\lambda}{960} \sum\limits_x \tr\lr{\phi_x^2} \tr\lr{\phi_x^2} 
\end{eqnarray} 

\begin{eqnarray}
\label{double_trace_derivative}
 \frac{\partial}{\partial \phi}
 \sum\limits_{l=1}^{k} \mathcal{J}_{k+1,l} 
 \tr\lr{\phi^{2 l}} \tr\lr{\phi^{2 k + 2 - 2 l}}
 =
 2 \sum\limits_{l=1}^k \mathcal{J}_{k+1,l} \, 2 l \, \phi^{2 l - 1} \tr\lr{\phi^{2 k + 2 - 2 l}}
\end{eqnarray}

\section{One-link action with exponential mapping}
\label{sec:one_link}

For the one-link action we get the simple expansion
\begin{eqnarray}
\label{single_link_action}
 \frac{N}{\lambda} \tr\lr{2 - e^{i \alpha \phi} - e^{-i \alpha \phi}}
 =
 \sum\limits_{k=1}^{+\infty} \lr{-1}^{k-1} \frac{2 N \alpha^{2 k}}{\lambda \, \lr{2 k}!} \tr{\phi^{2 k}}
 =
 \frac{N \alpha^2}{\lambda} \tr{\phi^2} + \ldots
\end{eqnarray}
We now choose the value of $\alpha$ in such a way that the coefficient of $\tr\phi^2$ in the action is $1/2$: $\alpha^2 = \frac{6 \lambda}{12 + \lambda}$. Another useful relation is $\frac{1}{\lambda} = \frac{1}{2 \alpha^2} - \frac{1}{12}$.

In the end, we can write the action as
\begin{eqnarray}
\label{action_general}
 S\lrs{\phi} = \frac{N}{2} \tr{\phi^2}
 +
 N \sum\limits_{k=1}^{+\infty} \alpha^{2 k} \mathcal{S}_k \tr{\phi^{2 k + 2}}
 + %\nonumber \\ +
 \sum\limits_{k,l=1}^{+\infty} \alpha^{2 \lr{k + l}} \mathcal{D}_{k,l} \tr{\phi^{2 k}} \tr{\phi^{2 l}} ,
\end{eqnarray}
where
\begin{eqnarray}
\label{vertices_explicit}
 \mathcal{S}_k = \ldots
 \nonumber \\
 \mathcal{D}_{k,l} = \ldots
\end{eqnarray}

The derivative of this action is
\begin{eqnarray}
\label{action_general_derivative}
 \frac{\partial S\lrs{\phi}}{\partial \phi} =
 N \phi
 +
 \sum\limits_{k=1}^{+\infty} \alpha^{2 k} \mathcal{S}_k \lr{2 k + 2} \phi^{2 k + 1}
 + %\nonumber \\ +
 2 \sum\limits_{k,l=1}^{+\infty} \alpha^{2 \lr{k + l}} \lr{2 k} \mathcal{D}_{k,l} \phi^{2 k - 1} \tr{\phi^{2 l}}
 = \nonumber \\ =
 N \phi
 -
 \sum\limits_{k=1}^{+\infty} \alpha^{2 k} \bar{\mathcal{S}}_k \phi^{2 k + 1}
 - %\nonumber \\ +
 \sum\limits_{k,l=1}^{+\infty} \alpha^{2 \lr{k + l}} \bar{\mathcal{D}}_{k,l} \phi^{2 k - 1} \tr{\phi^{2 l}}
\end{eqnarray}

\section{Schwinger-Dyson equations for the one-link action}

\end{document}
